refactor(library/init/meta): remove whnf_core

src/library/tactic/tactic_state.cpp
@@ -431,7 +431,7 @@ vm_obj tactic_infer_type(vm_obj const & e, vm_obj const & s0) {
     }
 }
 
-vm_obj tactic_whnf_core(vm_obj const & t, vm_obj const & e, vm_obj const & s0) {
+vm_obj tactic_whnf(vm_obj const & e, vm_obj const & t, vm_obj const & s0) {
     tactic_state const & s = to_tactic_state(s0);
     type_context ctx       = mk_type_context_for(s, to_transparency_mode(t));
     try {
@@ -806,7 +806,7 @@ void initialize_tactic_state() {
     DECLARE_VM_BUILTIN(name({"tactic", "result"}),               tactic_result);
     DECLARE_VM_BUILTIN(name({"tactic", "format_result"}),        tactic_format_result);
     DECLARE_VM_BUILTIN(name({"tactic", "infer_type"}),           tactic_infer_type);
-    DECLARE_VM_BUILTIN(name({"tactic", "whnf_core"}),            tactic_whnf_core);
+    DECLARE_VM_BUILTIN(name({"tactic", "whnf"}),                 tactic_whnf);
     DECLARE_VM_BUILTIN(name({"tactic", "is_def_eq"}),            tactic_is_def_eq);
     DECLARE_VM_BUILTIN(name({"tactic", "eta_expand"}),           tactic_eta_expand);
     DECLARE_VM_BUILTIN(name({"tactic", "eta"}),                  tactic_eta);
