tests/lean/whnf_core1.lean
@@ -9,6 +9,6 @@ example (a : nat) : true :=
 by do
   to_expr `(f a) >>= whnf >>= trace,
   to_expr `(g a) >>= whnf >>= trace,
-  to_expr `(f a) >>= whnf_core reducible >>= trace,
-  to_expr `(g a) >>= whnf_core reducible >>= trace,
+  to_expr `(f a) >>= (λ e, whnf e reducible) >>= trace,
+  to_expr `(g a) >>= (λ e, whnf e reducible) >>= trace,
   constructor
